proved most generality of iter_step

trunk/color/Term/WithArity/AUnif.v
@@ -7,7 +7,7 @@ See the COPYRIGHTS and LICENSE files.
 syntactic unification
 *)
 
-(* $Id: AUnif.v,v 1.2 2008-05-15 15:40:04 blanqui Exp $ *)
+(* $Id: AUnif.v,v 1.3 2008-05-18 13:07:46 blanqui Exp $ *)
 
 Set Implicit Arguments.
 
@@ -24,10 +24,15 @@ Notation substitution := (substitution Sig).
 Ltac case_symb_eq f g := case_beq (@beq_symb_ok Sig) (@beq_symb Sig f g).
 
 (***********************************************************************)
-(* equations *)
+(* unification problem *)
 
 Notation eqn := ((term * term)%type).
 Notation eqns := (list eqn).
+
+Notation solved_eqn := ((variable * term)%type).
+Notation solved_eqns := (list solved_eqn).
+
+Notation problem := (option ((solved_eqns * eqns)%type)).
 
 Definition eqn_app s (e : eqn) := (app s (fst e), app s (snd e)).
 
@@ -64,6 +69,25 @@ unfold vars_eqn. simpl.
 transitivity (union (union (vars x) (vars a)) (union (vars_terms ts) (vars_terms us))). apply union_m. refl. apply IHus. Equal; union.
 Qed.
 
+Lemma mem_vars_app_single : forall n (u : term) x v,
+  mem n (vars u) = false -> mem n (vars v) = false ->
+  mem n (vars (app (single x v) u)) = false.
+
+Proof.
+intros. transitivity (mem n (if mem x (vars u) then union (vars v) (remove x (vars u)) else vars u)). apply mem_m. refl. apply vars_subs.
+case_eq (mem x (vars u)). mem. rewrite H0. rewrite H. refl.
+hyp.
+Qed.
+
+Lemma mem_vars_app_single' : forall n (u v : term),
+  mem n (vars v) = false -> mem n (vars (app (single n v) u)) = false.
+
+Proof.
+intros. transitivity (mem n (if mem n (vars u) then union (vars v) (remove n (vars u)) else vars u)). apply mem_m. refl. apply vars_subs.
+case_eq (mem n (vars u)). mem. rewrite H0. rewrite H. refl.
+hyp.
+Qed.
+
 Lemma vars_eqn_subs : forall x v e,
   vars_eqn (eqn_app (single x v) e) [=]
   if mem x (vars_eqn e) then union (vars v) (remove x (vars_eqn e))
@@ -71,8 +95,8 @@ Lemma vars_eqn_subs : forall x v e,
 
 Proof.
 intros. destruct e as [l r]. unfold vars_eqn, eqn_app. simpl.
-(*FIXME*)transitivity (union (if mem x (vars l) then union (vars v) (remove x (vars l)) else vars l) (if mem x (vars r) then union (vars v) (remove x (vars r)) else vars r)). apply union_m; apply vars_subs. autorewrite with mem.
-case_eq (mem x (vars l)); case_eq (mem x (vars r)); autorewrite with bool.
+transitivity (union (if mem x (vars l) then union (vars v) (remove x (vars l)) else vars l) (if mem x (vars r) then union (vars v) (remove x (vars r)) else vars r)). apply union_m; apply vars_subs. mem.
+case_eq (mem x (vars l)); case_eq (mem x (vars r)); bool.
 transitivity (union (vars v) (union (remove x (vars l)) (remove x (vars r)))).
 apply union_idem_3. apply union_m. refl. symmetry. apply remove_union.
 transitivity (union (vars v) (union (remove x (vars l)) (vars r))).
@@ -93,12 +117,11 @@ Lemma vars_eqns_subs : forall x v l,
     else vars_eqns l.
 
 Proof.
-induction l; simpl; intros. refl. autorewrite with mem.
-(*FIXME*)transitivity (union (if mem x (vars_eqn a) then union (vars v) (remove x (vars_eqn a)) else vars_eqn a) (if mem x (vars_eqns l)
+induction l; simpl; intros. refl. mem.
+transitivity (union (if mem x (vars_eqn a) then union (vars v) (remove x (vars_eqn a)) else vars_eqn a) (if mem x (vars_eqns l)
           then union (vars v) (remove x (vars_eqns l))
           else vars_eqns l)). apply union_m. apply vars_eqn_subs. exact IHl.
-case_eq (mem x (vars_eqn a)); case_eq (mem x (vars_eqns l));
-  autorewrite with bool.
+case_eq (mem x (vars_eqn a)); case_eq (mem x (vars_eqns l)); bool.
 transitivity (union (vars v) (union (remove x (vars_eqn a)) (remove x (vars_eqns l)))). apply union_idem_3. apply union_m. refl. symmetry. apply remove_union.
 transitivity (union (vars v) (union (remove x (vars_eqn a)) (vars_eqns l))).
 apply union_assoc. apply union_m. refl.
@@ -115,21 +138,21 @@ Qed.
 (***********************************************************************)
 (** well-formed unification problems *)
 
-Notation solved_eqn := ((variable * term)%type).
-Notation solved_eqns := (list solved_eqn).
-Notation problem := (option ((solved_eqns * eqns)%type)).
-
 Definition notin_eqn x (e : eqn) :=
   mem x (vars (fst e)) = false /\ mem x (vars (snd e)) = false.
 
 Definition notin_solved_eqn x (e : solved_eqn) :=
   x <> fst e /\ mem x (vars (snd e)) = false.
 
+Definition notin_vars_solved_eqn (v : term) (e : solved_eqn) :=
+  mem (fst e) (vars v) = false.
+
 Fixpoint solved_eqns_wf (l : solved_eqns) :=
   match l with
     | nil => True
     | (x, v) :: l' => mem x (vars v) = false
       /\ lforall (notin_solved_eqn x) l' /\ solved_eqns_wf l'
+      /\ lforall (notin_vars_solved_eqn v) l'
   end.
 
 Definition notin l2 (e : solved_eqn) := lforall (notin_eqn (fst e)) l2.
@@ -151,10 +174,9 @@ Lemma lforall_notin_solved_eqn_1 : forall n t, mem n (vars t) = false ->
 
 Proof.
 induction l; simpl. auto. destruct a. simpl. unfold notin_eqn. simpl.
-autorewrite with mem. intros. unfold notin_solved_eqn. simpl. intuition.
+mem. intros. unfold notin_solved_eqn. simpl. intuition.
 subst n0. rewrite (beq_refl beq_nat_ok) in H4. discriminate.
-transitivity (mem n (if mem n (vars t1) then union (vars t0) (remove n (vars t1)) else vars t1)). apply mem_m. refl. apply vars_subs.
-case_eq (mem n (vars t1)). autorewrite with mem bool. hyp. hyp.
+apply mem_vars_app_single'; hyp.
 Qed.
 
 Lemma lforall_notin_solved_eqn_1' : forall n t, mem n (vars t) = false ->
@@ -163,23 +185,63 @@ Lemma lforall_notin_solved_eqn_1' : forall n t, mem n (vars t) = false ->
 
 Proof.
 induction l; simpl. auto. destruct a. simpl. unfold notin_eqn. simpl.
-autorewrite with mem. intros. unfold notin_solved_eqn. simpl. intuition.
+mem. intros. unfold notin_solved_eqn. simpl. intuition.
 subst n0. rewrite (beq_refl beq_nat_ok) in H1. discriminate.
-transitivity (mem n (if mem n (vars t1) then union (vars t0) (remove n (vars t1)) else vars t1)). apply mem_m. refl. apply vars_subs.
-case_eq (mem n (vars t1)). autorewrite with mem bool. hyp. hyp.
+apply mem_vars_app_single'; hyp.
 Qed.
 
 Lemma lforall_notin_solved_eqn_2 : forall n t, mem n (vars t) = false ->
-  forall x, beq_nat x n = false ->
-    forall l, lforall (notin_solved_eqn n) l -> 
+  forall x l, lforall (notin_solved_eqn n) l -> 
       lforall (notin_solved_eqn n) (map (solved_eqn_app (single x t)) l).
 
 Proof.
-induction l; simpl. auto. destruct a. intuition. unfold notin_solved_eqn in H2.
-simpl in H2. unfold notin_solved_eqn. simpl. intuition.
-transitivity (mem n (if mem x (vars t1) then union (vars t0) (remove x (vars t1)) else vars t1)). apply mem_m. refl. apply vars_subs.
-case_eq (mem x (vars t1)). autorewrite with mem. rewrite H0. rewrite H5.
-rewrite H. refl. hyp.
+induction l; simpl. auto. destruct a. intuition. unfold notin_solved_eqn in H1.
+simpl in H1. unfold notin_solved_eqn. simpl. intuition.
+apply mem_vars_app_single; hyp.
+Qed.
+
+Lemma lforall_notin_vars_solved_eqn_1 : forall n t0 t1 l' l,
+  lforall (notin ((Var n, t0) :: l')) l ->
+  lforall (notin_vars_solved_eqn t1) l ->
+  lforall (notin_vars_solved_eqn (app (single n t0) t1))
+  (map (solved_eqn_app (single n t0)) l).
+
+Proof.
+induction l; simpl. auto. destruct a.
+unfold solved_eqn_app at 1, notin_vars_solved_eqn at 1 3, notin_eqn. simpl.
+intuition. apply mem_vars_app_single; hyp.
+Qed.
+
+Lemma lforall_notin_vars_solved_eqn_1' : forall n t0 t1 l' l,
+  lforall (notin ((t0, Var n) :: l')) l ->
+  lforall (notin_vars_solved_eqn t1) l ->
+  lforall (notin_vars_solved_eqn (app (single n t0) t1))
+  (map (solved_eqn_app (single n t0)) l).
+
+Proof.
+induction l; simpl. auto. destruct a.
+unfold solved_eqn_app at 1, notin_vars_solved_eqn at 1 3, notin_eqn. simpl.
+intuition. apply mem_vars_app_single; hyp.
+Qed.
+
+Lemma lforall_notin_vars_solved_eqn_2 : forall n u l' l,
+  lforall (notin ((Var n, u) :: l')) l ->
+  lforall (notin_vars_solved_eqn u) (map (solved_eqn_app (single n u)) l).
+
+Proof.
+induction l; simpl. auto. destruct a.
+unfold notin_vars_solved_eqn at 1, notin_eqn, notin at 1. simpl.
+mem. intuition.
+Qed.
+
+Lemma lforall_notin_vars_solved_eqn_2' : forall n u l' l,
+  lforall (notin ((u, Var n) :: l')) l ->
+  lforall (notin_vars_solved_eqn u) (map (solved_eqn_app (single n u)) l).
+
+Proof.
+induction l; simpl. auto. destruct a.
+unfold notin_vars_solved_eqn at 1, notin_eqn, notin at 1. simpl.
+mem. intuition.
 Qed.
 
 Lemma solved_eqns_wf_map : forall n t, mem n (vars t) = false ->
@@ -188,10 +250,9 @@ Lemma solved_eqns_wf_map : forall n t, mem n (vars t) = false ->
 
 Proof.
 induction l; simpl. auto. destruct a. simpl. unfold notin_eqn. simpl.
-autorewrite with mem. intuition.
-transitivity (mem n0 (if mem n (vars t1) then union (vars t0) (remove n (vars t1)) else vars t1)). apply mem_m. refl. apply vars_subs.
-case_eq (mem n (vars t1)). autorewrite with mem. rewrite H7. rewrite H2.
-rewrite H0. refl. hyp. apply lforall_notin_solved_eqn_2; hyp.
+mem. intuition.
+apply mem_vars_app_single; hyp. apply lforall_notin_solved_eqn_2; hyp.
+apply lforall_notin_vars_solved_eqn_1 with l'; hyp.
 Qed.
 
 Lemma solved_eqns_wf_map' : forall n t, mem n (vars t) = false ->
@@ -200,10 +261,9 @@ Lemma solved_eqns_wf_map' : forall n t, mem n (vars t) = false ->
 
 Proof.
 induction l; simpl. auto. destruct a. simpl. unfold notin_eqn. simpl.
-autorewrite with mem. intuition.
-transitivity (mem n0 (if mem n (vars t1) then union (vars t0) (remove n (vars t1)) else vars t1)). apply mem_m. refl. apply vars_subs.
-case_eq (mem n (vars t1)). autorewrite with mem. rewrite H7. rewrite H2.
-rewrite H0. refl. hyp. apply lforall_notin_solved_eqn_2; hyp.
+mem. intuition.
+apply mem_vars_app_single; hyp. apply lforall_notin_solved_eqn_2; hyp.
+apply lforall_notin_vars_solved_eqn_1' with l'; hyp.
 Qed.
 
 Lemma notin_map : forall x t, mem x (vars t) = false ->
@@ -212,27 +272,26 @@ Lemma notin_map : forall x t, mem x (vars t) = false ->
 Proof.
 induction l; simpl. trivial. destruct a. unfold notin_eqn. simpl. intuition.
 transitivity (mem x (if mem x (vars t1) then union (vars t0) (remove x (vars t1)) else vars t1)). apply mem_m. refl. apply vars_subs.
-case_eq (mem x (vars t1)). autorewrite with mem. rewrite H. rewrite H0.
+case_eq (mem x (vars t1)). mem. rewrite H. rewrite H0.
 refl. hyp.
 transitivity (mem x (if mem x (vars t2) then union (vars t0) (remove x (vars t2)) else vars t2)). apply mem_m. refl. apply vars_subs.
-case_eq (mem x (vars t2)). autorewrite with mem. rewrite H. rewrite H0.
+case_eq (mem x (vars t2)). mem. rewrite H. rewrite H0.
 refl. hyp.
 Qed.
 
 Lemma lforall_notin_eqn : forall x t, mem x (vars t) = false ->
-  forall n, beq_nat n x = false ->
-    forall l, lforall (notin_eqn x) l ->
+  forall n l, lforall (notin_eqn x) l ->
       lforall (notin_eqn x) (map (eqn_app (single n t)) l).
 
 Proof.
 induction l; simpl; intuition. destruct a. unfold eqn_app. simpl.
-unfold notin_eqn. simpl. unfold notin_eqn in H2. simpl in H2. intuition.
+unfold notin_eqn. simpl. unfold notin_eqn in H1. simpl in H1. intuition.
 transitivity (mem x (if mem n (vars t1) then union (vars t0) (remove n (vars t1)) else vars t1)). apply mem_m. refl. apply vars_subs.
-case_eq (mem n (vars t1)). autorewrite with mem. rewrite H. rewrite H0.
-rewrite H4. refl. hyp.
+case_eq (mem n (vars t1)). mem. rewrite H. rewrite H3. refl.
+hyp.
 transitivity (mem x (if mem n (vars t2) then union (vars t0) (remove n (vars t2)) else vars t2)). apply mem_m. refl. apply vars_subs.
-case_eq (mem n (vars t2)). autorewrite with mem. rewrite H. rewrite H0.
-rewrite H5. refl. hyp.
+case_eq (mem n (vars t2)). mem. rewrite H. rewrite H4. refl.
+hyp.
 Qed.
 
 Lemma lforall_notin : forall x t l' l,
@@ -242,7 +301,7 @@ Lemma lforall_notin : forall x t l' l,
 
 Proof.
 induction l; simpl. auto. destruct a. simpl. unfold notin_eqn. simpl.
-autorewrite with mem. intuition. unfold notin. simpl.
+mem. intuition. unfold notin. simpl.
 unfold notin in H2. simpl in H2. apply lforall_notin_eqn; hyp.
 Qed.
 
@@ -253,7 +312,7 @@ Lemma lforall_notin' : forall x t l' l,
 
 Proof.
 induction l; simpl. auto. destruct a. simpl. unfold notin_eqn. simpl.
-autorewrite with mem. intuition. unfold notin. simpl.
+mem. intuition. unfold notin. simpl.
 unfold notin in H2. simpl in H2. apply lforall_notin_eqn; hyp.
 Qed.
 
@@ -280,7 +339,12 @@ Definition step (p : problem) :=
   match p with
     | Some (l1, e :: l2) =>
       match e with
-        | (v, Var x) | (Var x, v) =>
+        | (v, Var x) =>
+          if beq_term v (Var x) then Some (l1, l2)
+            else if mem x (vars v) then None
+              else Some ((x, v) :: List.map (solved_eqn_app (single x v)) l1,
+              List.map (eqn_app (single x v)) l2)
+        | (Var x, v) =>
           if beq_term v (Var x) then Some (l1, l2)
             else if mem x (vars v) then None
               else Some ((x, v) :: List.map (solved_eqn_app (single x v)) l1,
@@ -296,7 +360,7 @@ Definition step (p : problem) :=
 Fixpoint iter_step k (p : problem) {struct k} :=
   match k with
     | 0 => p
-    | S k' => iter_step k' (step p)
+    | S k' => step (iter_step k' p)
   end.
 
 (***********************************************************************)
@@ -308,36 +372,42 @@ Proof.
 intro. destruct p. 2: auto. destruct p. destruct l0. auto. destruct p.
 destruct t0; destruct t1.
 (* var-var *)
-simpl. autorewrite with mem. case_nat_eq n n0; simpl.
+simpl. mem. case_nat_eq n n0; simpl.
 intuition. gen H1. elim l; simpl; intuition.
-autorewrite with mem. rewrite H. intuition.
-eapply lforall_notin_solved_eqn_1. simpl. autorewrite with mem. hyp.
-apply H2.
-eapply solved_eqns_wf_map'. simpl. autorewrite with mem. hyp.
-hyp. apply H2.
-apply notin_map. simpl. autorewrite with mem. hyp.
+mem. rewrite H. intuition.
+eapply lforall_notin_solved_eqn_1. simpl. mem. hyp. apply H2.
+eapply solved_eqns_wf_map'. simpl. mem. hyp. hyp. apply H2.
+gen H2. elim l; simpl; intuition. unfold notin_vars_solved_eqn. simpl.
+unfold notin_eqn in H2. simpl in H2. intuition.
+apply notin_map. simpl. mem. hyp.
 apply lforall_notin. hyp.
 (* var-fun *)
-Opaque vars. simpl. rewrite vars_fun. intuition.
-case_eq (mem n (vars_terms v)). simpl. trivial.
-simpl. rewrite vars_fun. intuition.
-eapply lforall_notin_solved_eqn_1'. rewrite vars_fun. hyp. apply H1.
-eapply solved_eqns_wf_map. rewrite vars_fun. hyp. hyp. apply H1.
-apply notin_map. rewrite vars_fun. hyp.
+Opaque vars. simpl. set (u := Fun f v). intuition.
+case_eq (mem n (vars u)); simpl; intuition.
+eapply lforall_notin_solved_eqn_1'. hyp. apply H1.
+eapply solved_eqns_wf_map. hyp. hyp. apply H1.
+apply lforall_notin_vars_solved_eqn_2 with l0. hyp.
+apply notin_map. hyp.
 apply lforall_notin'. hyp.
-(* fun-var *)
-simpl. rewrite vars_fun. intuition.
-case_eq (mem n (vars_terms v)). simpl. trivial.
-simpl. rewrite vars_fun. intuition.
-eapply lforall_notin_solved_eqn_1. rewrite vars_fun. hyp. apply H1.
-eapply solved_eqns_wf_map'. rewrite vars_fun. hyp. hyp. apply H1.
-apply notin_map. rewrite vars_fun. hyp.
+(* fun-var *) (* about the same proof *)
+simpl. set (u := Fun f v). intuition.
+case_eq (mem n (vars u)); simpl; intuition.
+eapply lforall_notin_solved_eqn_1. hyp. apply H1.
+eapply solved_eqns_wf_map'. hyp. hyp. apply H1.
+apply lforall_notin_vars_solved_eqn_2' with l0. hyp.
+apply notin_map. hyp.
 apply lforall_notin. hyp.
 (* fun-fun *)
 simpl. case_symb_eq f f0; simpl; intuition.
 gen H1. elim l; simpl; intuition. gen H1. unfold notin_eqn. simpl.
 do 2 rewrite vars_fun. gen H4. unfold notin. simpl. rewrite lforall_app.
 intuition. apply lforall_notin_eqn_combine; hyp. Transparent vars.
+Qed.
+
+Lemma iter_step_wf : forall p k, problem_wf p -> problem_wf (iter_step k p).
+
+Proof.
+induction k; simpl; intuition. apply step_wf. hyp.
 Qed.
 
 (***********************************************************************)
@@ -396,8 +466,8 @@ rewrite H3. rewrite app_app. apply app_eq. intros.
 unfold comp, single. case_nat_eq n x; auto.
 Qed.
 
-Lemma app_comp_single : forall s x u, s x = app s u ->
-  forall t : term, app (comp s (single x u)) t = app s t.
+Lemma app_comp_single : forall s x (u : term), s x = app s u ->
+  forall t, app (comp s (single x u)) t = app s t.
 
 Proof.
 intros. set (s' := comp s (single x u)). pattern t0.
@@ -448,7 +518,7 @@ Proof.
 intros s p. destruct p. 2: simpl; intuition. destruct p. destruct l0.
 simpl. intuition. destruct p. destruct t0; destruct t1.
 (* var-var *)
-simpl. unfold is_sol_eqn. autorewrite with mem. simpl.
+simpl. unfold is_sol_eqn. mem. simpl.
 case_nat_eq n n0; simpl. intuition. unfold is_sol_solved_eqn. simpl. intuition.
 rewrite is_sol_solved_eqns_map; auto. rewrite is_sol_eqns_map; auto.
 rewrite is_sol_solved_eqns_map in H3; auto. rewrite is_sol_eqns_map in H2; auto.
@@ -477,16 +547,189 @@ apply args_eq. hyp. intuition; try contradiction. Funeqtac.
 rewrite (beq_refl beq_symb_ok) in H. discriminate. Transparent vars.
 Qed.
 
+Lemma iter_step_correct_complete : forall s p k,
+  is_sol s p <-> is_sol s (iter_step k p).
+
+Proof.
+induction k; simpl. intuition. rewrite <- step_correct_complete. hyp.
+Qed.
+
+(***********************************************************************)
+(** extension of a substitution *)
+
+Definition extend (s : substitution) x v : substitution :=
+  fun y => if beq_nat y x then v else s y.
+
+Lemma app_extend_notin : forall s x v u,
+  mem x (vars u) = false -> app (extend s x v) u = app s u.
+
+Proof.
+intros s x v u. set (s' := extend s x v). pattern u.
+apply term_ind with (Q := fun n (us : terms n) =>
+  mem x (vars_terms us) = false -> Vmap (app s') us = Vmap (app s) us);
+  clear u.
+intro. simpl. mem. unfold s', extend.
+case (beq_nat x0 x). intro. discriminate. refl.
+intros f us. rewrite vars_fun. do 2 rewrite app_fun. intros. apply args_eq.
+auto. refl.
+intros u n us. simpl. mem. intros.
+destruct (orb_false_elim H1). apply Vcons_eq; intuition.
+Qed.
+Lemma is_sol_solved_eqns_extend : forall s n v l,
+  lforall (notin_solved_eqn n) l ->
+  is_sol_solved_eqns s l -> is_sol_solved_eqns (extend s n v) l.
+
+Proof.
+induction l; simpl. auto. destruct a.
+unfold notin_solved_eqn at 1, is_sol_solved_eqn. simpl. intuition.
+unfold extend at 1. case_nat_eq n0 n. change (n0<>n0) in H0. irrefl.
+rewrite H. symmetry. apply app_extend_notin. hyp.
+Qed.
+
 (***********************************************************************)
 (** substitution corresponding to solved equations *)
 
-Definition extend (s : substitution) x (v : term) : substitution :=
-  fun y => if beq_nat x y then v else s y.
+Notation id := (@id Sig).
 
 Fixpoint subst_of_solved_eqns (l : solved_eqns) :=
   match l with
     | (x, v) :: l' => extend (subst_of_solved_eqns l') x v
-    | nil => @id Sig
+    | nil => id
   end.
+
+Fixpoint dom (l : solved_eqns) :=
+  match l with
+    | (x, _) :: l' => add x (dom l')
+    | nil => empty
+  end.
+
+Lemma dom_subst_of_solved_eqns : forall x l,
+  mem x (dom l) = false -> subst_of_solved_eqns l x = Var x.
+
+Proof.
+induction l; simpl. mem. refl. destruct a.
+mem. intro. destruct (orb_false_elim H). unfold extend.
+rewrite (beq_com beq_nat_ok) in H0. rewrite H0. auto.
+Qed.
+
+Implicit Arguments dom_subst_of_solved_eqns [x l].
+
+Lemma lforall_notin_vars_solved_eqn_dom : forall x u l,
+  lforall (notin_vars_solved_eqn u) l ->
+  mem x (vars u) = true -> mem x (dom l) = false.
+
+Proof.
+induction l; simpl. mem. refl. destruct a.
+unfold notin_vars_solved_eqn at 1. simpl. mem. intuition.
+case_nat_eq n x; simpl. rewrite H1 in H0. discriminate. hyp.
+Qed.
+
+Implicit Arguments lforall_notin_vars_solved_eqn_dom [x u l].
+
+Lemma lforall_notin_vars_solved_eqn_mem : forall x u l,
+  lforall (notin_vars_solved_eqn u) l ->
+  mem x (dom l) = true -> mem x (vars u) = false.
+
+Proof.
+induction l. simpl. mem. intros. discriminate. destruct a. simpl. mem.
+unfold notin_vars_solved_eqn at 1. simpl. intuition.
+destruct (orb_true_elim H0). rewrite beq_nat_ok in e. subst n. hyp. auto.
+Qed.
+
+Implicit Arguments lforall_notin_vars_solved_eqn_mem [x u l].
+
+Lemma app_eq : forall s1 s2 (t : term),
+  (forall x, mem x (vars t) = true -> s1 x = s2 x) -> app s1 t = app s2 t.
+
+Proof.
+intros. apply app_eq. intro. rewrite in_vars_mem. auto.
+Qed.
+
+Lemma app_eq_id : forall s (t : term),
+  (forall x, mem x (vars t) = true -> s x = Var x) -> app s t = t.
+
+Proof.
+intros. apply app_eq_id. intro. rewrite in_vars_mem. auto.
+Qed.
+
+Lemma lforall_notin_solved_eqn_mem : forall n x l,
+  lforall (notin_solved_eqn n) l -> beq_nat x n = false ->
+  mem n (vars (subst_of_solved_eqns l x)) = false.
+
+Proof.
+induction l. simpl. mem. auto. simpl. destruct a. unfold notin_solved_eqn at 1.
+simpl. intuition. unfold extend. case_nat_eq x n0; hyp.
+Qed.
+
+Implicit Arguments lforall_notin_solved_eqn_mem [n x l].
+
+Lemma subst_of_solved_eqns_correct : forall l, solved_eqns_wf l ->
+  is_sol_solved_eqns (subst_of_solved_eqns l) l.
+
+Proof.
+induction l; simpl. auto. set (s := subst_of_solved_eqns l). destruct a.
+unfold is_sol_solved_eqn. simpl. intuition. unfold extend at 1. simpl.
+rewrite (beq_refl beq_nat_ok). rewrite app_extend_notin. 2: hyp.
+symmetry. apply app_eq_id. intros.
+ded (lforall_notin_vars_solved_eqn_dom H3 H4).
+ded (dom_subst_of_solved_eqns H5). hyp.
+apply is_sol_solved_eqns_extend; hyp.
+Qed.
+
+(***********************************************************************)
+(** most generality *)
+
+Definition theta l (s : substitution) y :=
+  if mem y (dom l) then Var y else s y.
+
+Lemma subst_of_solved_eqns_most_general :
+  forall s l, solved_eqns_wf l -> is_sol_solved_eqns s l ->
+    forall x, s x = app (theta l s) (subst_of_solved_eqns l x).
+
+Proof.
+induction l. refl. destruct a. unfold is_sol_solved_eqns. simpl.
+unfold is_sol_solved_eqn at 1. simpl. intuition. unfold extend.
+case_nat_eq x n. rewrite H. apply app_eq. intros. unfold theta. simpl. mem.
+case_nat_eq x x0; simpl. rewrite H1 in H4. discriminate.
+case_eq (mem x0 (dom l)). ded (lforall_notin_vars_solved_eqn_mem H5 H8).
+rewrite H4 in H9. discriminate. refl. rewrite H6. apply app_eq. intros.
+unfold theta. simpl. mem. case_nat_eq n x0. simpl.
+ded (lforall_notin_solved_eqn_mem H0 H4). rewrite H7 in H8. discriminate.
+simpl. refl.
+Qed.
+
+Lemma iter_step_None : forall p k, iter_step k p = None -> forall s, ~is_sol s p.
+
+Proof.
+intros. intro. rewrite (iter_step_correct_complete s p k) in H0. rewrite H in H0.
+hyp.
+Qed.
+
+Lemma iter_step_solved_eqn_wf : forall p l k, problem_wf p ->
+  iter_step k p = Some (l, nil) -> solved_eqns_wf l.
+
+Proof.
+intros. ded (iter_step_wf p k H). rewrite H0 in H1. simpl in H1. intuition.
+Qed.
+
+Lemma iter_step_Some : forall p l k, problem_wf p ->
+  iter_step k p = Some (l, nil) -> is_sol (subst_of_solved_eqns l) p.
+
+Proof.
+intros. rewrite (iter_step_correct_complete (subst_of_solved_eqns l) p k).
+rewrite H0. simpl. intuition. apply subst_of_solved_eqns_correct.
+eapply iter_step_solved_eqn_wf; eassumption.
+Qed.
+
+Lemma iter_step_most_general : forall p l k, problem_wf p ->
+  iter_step k p = Some (l, nil) -> forall s, is_sol s p ->
+    forall x, s x = app (theta l s) (subst_of_solved_eqns l x).
+
+Proof.
+intros. apply subst_of_solved_eqns_most_general.
+eapply iter_step_solved_eqn_wf; eassumption.
+cut (is_sol s (Some (l, nil))). simpl. intuition.
+rewrite <- H0. rewrite <- iter_step_correct_complete. hyp.
+Qed.
 
 End S.
