trunk/color/Term/WithArity/AVariables.v
@@ -7,7 +7,7 @@ See the COPYRIGHTS and LICENSE files.
 set of variables occuring in a term
 *)
 
-(* $Id: AVariables.v,v 1.1 2008-05-15 14:46:03 blanqui Exp $ *)
+(* $Id: AVariables.v,v 1.2 2008-05-18 13:07:46 blanqui Exp $ *)
 
 Set Implicit Arguments.
 
@@ -77,16 +77,33 @@ Fixpoint vars_list ts :=
     | t :: ts' => union (vars t) (vars_list ts')
   end.
 
+Lemma in_vars_mem : forall x (u : term),
+  List.In x (ATerm.vars u) <-> mem x (vars u) = true.
+
+Proof.
+intros. pattern u. apply term_ind with (Q := fun n (us : terms n) =>
+  List.In x (ATerm.vars_vec us) <-> mem x (vars_terms us) = true); clear u.
+intro. simpl. mem. intuition.
+intros f us H. rewrite ATerm.vars_fun. rewrite vars_fun. hyp.
+simpl. mem. intuition.
+intros. simpl. mem. intuition. destruct (in_app_or H0).
+ded (H1 H4). rewrite H5. refl. ded (H H4). rewrite H5. bool.
+refl. case (orb_true_elim H0); intro.
+ded (H2 e). apply in_appl. hyp. ded (H3 e). apply in_appr. hyp.
+Qed.
+
 Lemma mem_vars_terms : forall x n (ts : terms n),
   mem x (vars_terms ts) = true -> exists t, Vin t ts /\ mem x (vars t) = true.
 
 Proof.
-induction ts; simpl; autorewrite with mem; intuition. discriminate.
+induction ts; simpl; mem; intuition. discriminate.
 destruct (orb_true_elim H). exists a. auto.
 destruct (IHts e). exists x0. intuition.
 Qed.
 
 Implicit Arguments mem_vars_terms [x n ts].
+
+Open Scope nat_scope.
 
 Lemma mem_vars_size_app_ge : forall s x u,
   mem x (vars u) = true -> size (app s u) >= size (s x). 
@@ -95,10 +112,10 @@ Proof.
 intros s x u. pattern u. apply term_ind with (Q := fun n (ts : terms n) =>
   mem x (vars_terms ts) = true -> size_terms (Vmap (app s) ts) >= size (s x));
   clear u.
-intro. simpl. autorewrite with mem. intro. subst x0. omega.
+intro. simpl. mem. intro. subst x0. omega.
 intros f v. rewrite vars_fun. rewrite app_fun. rewrite size_fun. intros.
-ded (H H0). omega. simpl. autorewrite with mem. intros. discriminate.
-intros until v. simpl. autorewrite with mem. intros. destruct (orb_true_elim H1).
+ded (H H0). omega. simpl. mem. intros. discriminate.
+intros until v. simpl. mem. intros. destruct (orb_true_elim H1).
 ded (H e). omega. ded (H0 e). omega.
 Qed.
 
@@ -141,9 +158,9 @@ intros x v. apply term_ind with (Q := fun n (ts : terms n) =>
     else vars_terms ts).
 (* Var *)
 intro. simpl. unfold single. case_nat_eq x x0. autorewrite with mem Equal.
-(*FIXME*)transitivity (union (vars v) empty). symmetry. apply union_empty_right.
+transitivity (union (vars v) empty). symmetry. apply union_empty_right.
 apply union_m. refl. symmetry. apply remove_singleton.
-simpl. autorewrite with mem. rewrite (beq_com beq_nat_ok). rewrite H. refl.
+simpl. mem. rewrite (beq_com beq_nat_ok). rewrite H. refl.
 (* Fun *)
 intros. rewrite app_fun.
 coq_case_eq (mem x (vars (Fun f v0))); repeat rewrite vars_fun; intro;
@@ -151,8 +168,8 @@ coq_case_eq (mem x (vars (Fun f v0))); repeat rewrite vars_fun; intro;
 (* Vnil *)
 refl.
 (* Vcons *)
-intros u n us. simpl. autorewrite with mem. (*FIXME: rewrite H. rewrite H0.*)
-case_eq (mem x (vars u)); intro; autorewrite with bool.
+intros u n us. simpl. mem. (*FIXME: rewrite H. rewrite H0.*)
+case_eq (mem x (vars u)); intro; bool.
 case_eq (mem x (vars_terms us)); intros.
 transitivity (union (union (vars v) (remove x (vars u)))
   (union (vars v) (remove x (vars_terms us)))). apply union_m; hyp.
@@ -183,12 +200,11 @@ Lemma vars_subs_list : forall x v us,
     else vars_list us.
 
 Proof.
-induction us; simpl; intros. refl. autorewrite with mem.
-(*FIXME*)transitivity (union (if mem x (vars a) then union (vars v) (remove x (vars a)) else vars a) (if mem x (vars_list us)
+induction us; simpl; intros. refl. mem.
+transitivity (union (if mem x (vars a) then union (vars v) (remove x (vars a)) else vars a) (if mem x (vars_list us)
           then union (vars v) (remove x (vars_list us))
           else vars_list us)). apply union_m. apply vars_subs. exact IHus.
-case_eq (mem x (vars a)); case_eq (mem x (vars_list us)); intros;
-  autorewrite with bool.
+case_eq (mem x (vars a)); case_eq (mem x (vars_list us)); intros; bool.
 transitivity (union (vars v) (union (remove x (vars a)) (remove x (vars_list us)))). apply union_idem_3. apply union_m. refl. symmetry. apply remove_union.
 transitivity (union (vars v) (union (remove x (vars a)) (vars_list us))).
 apply union_assoc. apply union_m. refl.
